theories/solve_pure.v
@@ -3,190 +3,26 @@ From stdpp Require Import base.
 From cap_machine Require Import machine_base machine_parameters addr_reg solve_addr.
 From cap_machine Require Export solve_addr_extra classes class_instances.
 From cap_machine.rules Require Import rules_Get rules_AddSubLt.
+From machine_utils Require Export solve_pure.
 
-From Ltac2 Require Import Ltac2 Option.
-Set Default Proof Mode "Classic".
+Ltac solve_pure_addr := solve_pure_finz.
 
-(* The [solve_pure] tactic performs proof search to solve pure
-   capability-related side-goals. It handles goals involving:
+(* Extend the [solve_pure] tactic from [machine_utils] with additional hints
+   for solving goals specific to our machine, involving (additionally from what
+   [solve_pure] already handles):
 
-   - ContiguousRegion
-   - SubBounds
-   - InBounds
    - ExecPCPerm
    - PermFlows, PermFlowsTo  (TODO: extend)
    - decodeInstrW w = ?
-   - (a + z)%a = Some ?
    - readAllowed p (TODO: extend)
    - writeAllowed p (TODO: extend)
    - withinBounds (p, b, e, a) = true
    - is_Get
    - is_AddSubLt
-   - z_to_addr (z_of x) = ?
 
-   It also leverages the classes and instances defined in [classes.v] and
-   [class_instances.v], but those are not supposed to be used directly in proof
-   scripts: it is only expected that [solve_pure] internally generates
-   subgoals of these classes during proof search.
-
-   To extend [solve_pure]:
-   - prefer adding or using existing lemmas in [machine_base.v].
-   - only add lemmas in this file if they do not make sense in [machine_base.v]
-     (e.g. they involve some internal classes from [classes.v]).
-   - do register an appropriate [Hint Mode] in the [cap_pure] hint base for any
-     new notion you are adding support to.
-   - add hints to the [cap_pure] hint base for the relevant lemmas; be mindful
-     of proof search performance; do not register hints that could lead to a
-     blow up (including cases where the search fails). A typical example would
-     be adding a transitivity lemma as a hint.
-   - do add tests (see end of this file) for the kind of goals you are adding
-     support to.
-   - if needed, update the list of the supported types of goals above
-
-   Generally speaking, its important that the tactic is both fast when
-   succeeding and when failing.
-
-   /!\ Gotchas /!\:
-   - see the "Local context management" section below, regarding handling of
-     hypotheses from the local context; add [InCtx] hints if needed.
-   - do not add a [Hint Resolve] in [cap_pure] whose conclusion is a class from
-     [classes.v]. Register it as an instance instead, otherwise the Hint Modes
-     won't work as expected.
+   See the comments in [machine_utils/theories/solve_pure.v] on how to
+   extend [solve_pure] with more hints.
 *)
-
-(* Local context management
-
-   By default, [typeclasses eauto] will happily use any hypothesis from the
-   context to prove the goal, possibly wrongly instantiating evars.
-
-   To prevent that from happening, we first "freeze" the local context by
-   wrapping all hypotheses in [InCtx] before calling [typeclasses eauto].
-   Then, we have to register explicit hints to use hypotheses from the
-   local context, requiring a [InCtx ...].
-*)
-
-Class InCtx (P: Prop) := MkInCtx: P.
-
-Ltac freeze_hyps :=
-  repeat (match goal with
-  | h : ?P |- _ =>
-    lazymatch type of P with
-    | Prop => idtac
-    | _ => fail
-    end;
-    lazymatch P with
-    | InCtx _ => fail
-    | _ => idtac
-    end;
-    change P with (InCtx P) in h
-  end).
-
-Ltac unfreeze_hyps :=
-  unfold InCtx in *.
-
-(* Proof search features *)
-
-Create HintDb cap_pure discriminated.
-
-(* ContiguousRegion *)
-#[export] Hint Mode ContiguousRegion + - : cap_pure.
-
-Lemma ContiguousRegion_InCtx a z :
-  InCtx (ContiguousRegion a z) → ContiguousRegion a z.
-Proof. auto. Qed.
-#[export] Hint Resolve ContiguousRegion_InCtx : cap_pure.
-
-Instance IncrAddr_of_ContiguousRegion a z :
-  ContiguousRegion a z →
-  IncrAddr a z (a ^+ z)%a.
-Proof. intros [? ?]. unfold IncrAddr. solve_addr. Qed.
-
-Instance IncrAddr_in_ContiguousRegion (a a': Addr) (z o z' z'': Z) :
-  AsWeakAddrIncr a' a z →
-  ContiguousRegion a z'' →
-  CbvTC (z + o)%Z z' →
-  AddrOffsetLe 0 z →
-  AddrOffsetLe 0 o →
-  AddrOffsetLe z' z'' →
-  IncrAddr a' o (a ^+ z')%a.
-Proof.
-  unfold AsWeakAddrIncr, ContiguousRegion, CbvTC, AddrOffsetLe, IncrAddr.
-  intros -> [? ?] <- ? ?. solve_addr.
-Qed.
-
-(* SubBounds *)
-#[export] Hint Mode SubBounds + + - - : cap_pure.
-
-Lemma SubBounds_InCtx b e b' e' :
-  InCtx (SubBounds b e b' e') → SubBounds b e b' e'.
-Proof. auto. Qed.
-
-#[export] Hint Extern 2 (SubBounds _ _ ?b' ?e') =>
-  (is_evar b'; is_evar e'; apply SubBounds_InCtx) : cap_pure.
-
-#[export] Hint Extern 0 (SubBounds _ _ ?b' ?e') =>
-  (without_evars b'; without_evars e';
-   apply SubBounds_InCtx) : cap_pure.
-
-(* Consequences of SubBounds in terms of AddrLe/AddrLt *)
-
-(* TODO: figure out if these hints are actually exercised *)
-(* TODO: change these hints to lookup a SubBounds in the local context only *)
-
-Instance SubBounds_le_b_b' b e b' e' :
-  SubBounds b e b' e' →
-  AddrLe b b'.
-Proof. unfold SubBounds, AddrLe. solve_addr. Qed.
-
-Instance SubBounds_le_b'_e' b e b' e' :
-  SubBounds b e b' e' →
-  AddrLe b' e'.
-Proof. unfold SubBounds, AddrLe. solve_addr. Qed.
-
-Instance SubBounds_le_e_e' b e b' e' :
-  SubBounds b e b' e' →
-  AddrLe e' e.
-Proof. unfold SubBounds, AddrLe. solve_addr. Qed.
-
-
-(* Manually insert the transitive consequences from above, as we don't want to
-   have general transitivity instances for AddrLe/AddrLt *)
-
-Instance SubBounds_le_b_e' b e b' e' :
-  SubBounds b e b' e' →
-  AddrLe b e'.
-Proof. unfold SubBounds, AddrLe. solve_addr. Qed.
-
-Instance SubBounds_le_b_e b e b' e' :
-  SubBounds b e b' e' →
-  AddrLe b e.
-Proof. unfold SubBounds, AddrLe. solve_addr. Qed.
-
-Instance SubBounds_le_b'_e b e b' e' :
-  SubBounds b e b' e' →
-  AddrLe b' e.
-Proof. unfold SubBounds, AddrLe. solve_addr. Qed.
-
-(* transitivity to deduce lt of the outer bounds from lt of the inner bounds *)
-
-Instance SubBounds_lt_of_inner b e b' e' :
-  SubBounds b e b' e' →
-  AddrLt b' e' →
-  AddrLt b e.
-Proof. unfold SubBounds, AddrLt. solve_addr. Qed.
-
-(* InBounds *)
-
-#[export] Hint Mode InBounds + + + : cap_pure.
-
-#[export] Hint Resolve InBounds_sub : cap_pure.
-
-Lemma InBounds_compare (b a e: Addr) :
-  AddrLe b a →
-  AddrLt a e →
-  InBounds b e a.
-Proof. unfold AddrLe, AddrLt, InBounds. auto. Qed.
-#[export] Hint Resolve InBounds_compare : cap_pure.
 
 Lemma withinBounds_InCtx b e a :
   InCtx (withinBounds b e a = true) →
@@ -195,29 +31,13 @@ Proof.
   unfold InCtx, InBounds. cbn.
   intros [?%Z.leb_le ?%Z.ltb_lt]%andb_true_iff. solve_addr.
 Qed.
-#[export] Hint Resolve withinBounds_InCtx : cap_pure.
+#[export] Hint Resolve withinBounds_InCtx : solve_pure.
 
 (* isCorrectPC *)
 
-#[export] Hint Mode isCorrectPC + : cap_pure.
+#[export] Hint Mode isCorrectPC + : solve_pure.
 
-#[export] Hint Resolve isCorrectPC_ExecPCPerm_InBounds : cap_pure.
-
-(* IncrAddr *)
-
-(* This is just a proxy lemma, to then use the Hint Mode of IncrAddr. The
-   intention is that [a] and [z] are known, and that we want to infer [a']. *)
-Lemma IncrAddr_prove a z a' :
-  IncrAddr a z a' →
-  (a + z)%a = Some a'.
-Proof.
-  intros ->. reflexivity.
-Qed.
-#[export] Hint Resolve IncrAddr_prove : cap_pure.
-
-Instance IncrAddr_InCtx a z a' :
-  InCtx ((a + z)%a = Some a') → IncrAddr a z a'.
-Proof. auto. Qed.
+#[export] Hint Resolve isCorrectPC_ExecPCPerm_InBounds : solve_pure.
 
 (* Proxy lemma for DecodeInstr *)
 
@@ -227,32 +47,32 @@ Lemma DecodeInstr_prove `{MachineParameters} w i :
 Proof.
   intros ->. reflexivity.
 Qed.
-#[export] Hint Resolve DecodeInstr_prove : cap_pure.
+#[export] Hint Resolve DecodeInstr_prove : solve_pure.
 
 (* ExecPCPerm, PermFlows *)
 
-#[export] Hint Mode ExecPCPerm + : cap_pure.
-#[export] Hint Mode PermFlows - + : cap_pure.
+#[export] Hint Mode ExecPCPerm + : solve_pure.
+#[export] Hint Mode PermFlows - + : solve_pure.
 
 Lemma ExecPCPerm_InCtx p :
   InCtx (ExecPCPerm p) → ExecPCPerm p.
 Proof. auto. Qed.
-#[export] Hint Resolve ExecPCPerm_InCtx : cap_pure.
+#[export] Hint Resolve ExecPCPerm_InCtx : solve_pure.
 
-#[export] Hint Resolve ExecPCPerm_RX : cap_pure.
-#[export] Hint Resolve ExecPCPerm_RWX : cap_pure.
-#[export] Hint Resolve ExecPCPerm_not_E : cap_pure.
-#[export] Hint Resolve ExecPCPerm_flows_to : cap_pure.
+#[export] Hint Resolve ExecPCPerm_RX : solve_pure.
+#[export] Hint Resolve ExecPCPerm_RWX : solve_pure.
+#[export] Hint Resolve ExecPCPerm_not_E : solve_pure.
+#[export] Hint Resolve ExecPCPerm_flows_to : solve_pure.
 (* TODO: add a test checking the use of ExecPCPerm_flows_to (if it is still
    needed) *)
-#[export] Hint Resolve ExecPCPerm_readAllowed : cap_pure.
+#[export] Hint Resolve ExecPCPerm_readAllowed : solve_pure.
 (* Will only work if arguments are concrete terms *)
-#[export] Hint Extern 1 (readAllowed _ = true) => reflexivity : cap_pure.
-#[export] Hint Extern 1 (writeAllowed _ = true) => reflexivity : cap_pure.
-#[export] Hint Extern 1 (PermFlowsTo _ _ = true) => reflexivity : cap_pure.
+#[export] Hint Extern 1 (readAllowed _ = true) => reflexivity : solve_pure.
+#[export] Hint Extern 1 (writeAllowed _ = true) => reflexivity : solve_pure.
+#[export] Hint Extern 1 (PermFlowsTo _ _ = true) => reflexivity : solve_pure.
 (* Follows the same behavior as the Hint Mode for PermFlows *)
 #[export] Hint Extern 1 (PermFlowsTo ?p ?p' = true) =>
-  (without_evars p'; apply PermFlowsToReflexive): cap_pure.
+  (without_evars p'; apply PermFlowsToReflexive): solve_pure.
 
 (* withinBounds *)
 
@@ -262,87 +82,22 @@ Proof. auto. Qed.
    That's fine: this proxy lemma applies without risking instantiating any evar,
    and then the Hint Mode on [InBounds] can take effect. *)
 
-#[export] Hint Resolve withinBounds_InBounds : cap_pure.
+#[export] Hint Resolve withinBounds_InBounds : solve_pure.
 
 (* is_Get *)
-#[export] Hint Mode is_Get ! - - : cap_pure.
-#[export] Hint Resolve is_Get_GetP : cap_pure.
-#[export] Hint Resolve is_Get_GetB : cap_pure.
-#[export] Hint Resolve is_Get_GetE : cap_pure.
-#[export] Hint Resolve is_Get_GetA : cap_pure.
+#[export] Hint Mode is_Get ! - - : solve_pure.
+#[export] Hint Resolve is_Get_GetP : solve_pure.
+#[export] Hint Resolve is_Get_GetB : solve_pure.
+#[export] Hint Resolve is_Get_GetE : solve_pure.
+#[export] Hint Resolve is_Get_GetA : solve_pure.
 
 (* is_AddSubLt *)
-#[export] Hint Mode is_AddSubLt ! - - - : cap_pure.
-#[export] Hint Resolve is_AddSubLt_Add : cap_pure.
-#[export] Hint Resolve is_AddSubLt_Sub : cap_pure.
-#[export] Hint Resolve is_AddSubLt_Lt : cap_pure.
-
-(* z_to_addr *)
-
-(* Again, we go through a proxy lemma to be able to specify a Hint Mode on z/a
-   (see classes.v) *)
-
-Lemma z_to_addr_ZToAddr z a :
-  ZToAddr z a →
-  z_to_addr z = Some a.
-Proof. auto. Qed.
-
-#[export] Hint Resolve z_to_addr_ZToAddr : cap_pure.
-
-(* *)
-
-Ltac2 solve_pure () :=
-  first [ assumption
-    | discriminate
-    | ltac1:(freeze_hyps);
-      typeclasses_eauto with cap_pure typeclass_instances;
-      ltac1:(unfreeze_hyps) ].
-
-Ltac solve_pure :=
-  ltac2:(solve_pure ()).
-
-(* [solve_pure_addr]: solve_pure + hints to call [solve_addr]. Usually slow to
-   fail, should only be invoked manually. *)
-
-Create HintDb cap_pure_addr.
-
-Local Ltac hint_solve_addr := unfreeze_hyps; solve_addr.
-
-#[export] Hint Mode SubBounds + + + + : cap_pure_addr.
-#[export] Hint Extern 100 (SubBounds _ _ _ _) => hint_solve_addr : cap_pure_addr.
-
-#[export] Hint Mode InBounds + + + : cap_pure_addr.
-#[export] Hint Extern 100 (InBounds _ _ _) => hint_solve_addr : cap_pure_addr.
-
-#[export] Hint Mode IncrAddr + + + : cap_pure_addr.
-#[export] Hint Extern 100 (IncrAddr _ _ _) => hint_solve_addr : cap_pure_addr.
-
-Ltac solve_pure_addr :=
-  first [ assumption
-    | discriminate
-    | freeze_hyps;
-      typeclasses eauto with cap_pure cap_pure_addr typeclass_instances;
-      unfreeze_hyps ].
+#[export] Hint Mode is_AddSubLt ! - - - : solve_pure.
+#[export] Hint Resolve is_AddSubLt_Add : solve_pure.
+#[export] Hint Resolve is_AddSubLt_Sub : solve_pure.
+#[export] Hint Resolve is_AddSubLt_Lt : solve_pure.
 
 (* Tests *)
-
-Goal forall (b: Addr) a (z z': Z),
-  ContiguousRegion b z' →
-  AsWeakAddrIncr a b z →
-  AddrOffsetLt z z' →
-  AddrOffsetLe 0 z →
-  InBounds b (b ^+ z')%a a.
-Proof. intros. typeclasses eauto with cap_pure typeclass_instances. Qed.
-
-Goal forall (a: Addr),
-  ContiguousRegion a 5 →
-  exists a', IncrAddr a 1 a' ∧ a' = (a ^+ 1)%a.
-Proof. intros. eexists. split. solve_pure. reflexivity. Qed.
-
-Goal forall (a: Addr),
-  ContiguousRegion a 5 →
-  exists a', IncrAddr (a ^+ 1)%a 1 a' ∧ a' = (a ^+ 2)%a.
-Proof. intros. eexists. split. solve_pure. reflexivity. Qed.
 
 Goal forall (r_t1 PC: RegName) `{MachineParameters}, exists r1 r2,
   decodeInstrW (encodeInstrW (Mov r_t1 PC)) = Mov r1 r2 ∧
@@ -373,31 +128,5 @@ Goal forall (r_t1 r_t2 r_t3: RegName), exists r1 r2 r3,
   r1 = r_t2 ∧ r2 = r_t2 ∧ r3 = r_t3.
 Proof. do 3 eexists. repeat apply conj. solve_pure. all: reflexivity. Qed.
 
-Goal forall a, exists a',
-  ContiguousRegion a 2 →
-  ((a ^+ 1)%a + 1)%a = Some a' ∧ a' = (a ^+ 2)%a.
-Proof. intros. eexists. split. solve_pure. reflexivity. Qed.
-
-Goal forall (a b c: Addr),
-  (a + b)%a = Some c →
-  exists (a b c: Addr),
-  (a + b)%a = Some c.
-Proof. intros. do 3 eexists. Fail solve_pure. Abort.
-
-Goal forall (a b: Addr), exists c,
-  ContiguousRegion a 5 →
-  (a + (b - a))%a = Some c.
-Proof. intros. eexists. Fail solve_pure. Abort.
-
 Goal E ≠ RO. solve_pure. Qed.
 Goal forall (P: Prop), P → P. intros. solve_pure. Qed.
-
-Goal forall (a: Addr) z, exists z' a',
-  ContiguousRegion a z →
-  IncrAddr a z' a'.
-Proof. intros. do 2 eexists. intros. Fail solve_pure. Abort.
-
-(* Check that the hint corresponding to z_to_addr_z_of does not apply too
-   eagerly *)
-Goal exists a b, z_to_addr a = Some b.
-Proof. intros. do 2 eexists. Fail solve_pure. Abort.
