theories/class_instances.v
@@ -1,97 +1,9 @@
 From Coq Require Import ZArith Lia ssreflect.
 From stdpp Require Import base.
 From cap_machine Require Import machine_base machine_parameters addr_reg classes.
-
-(* Helper tactics *)
-
-#[export] Hint Extern 0 (@SimplTC _ _ _) => (cbn; reflexivity) : typeclass_instances.
-#[export] Hint Extern 0 (@CbvTC _ ?lhs _) => (
-  let lhs' := eval vm_compute in lhs in
-  change lhs with lhs';
-  reflexivity
-) : typeclass_instances.
-
-(* Address manipulation *)
-
-Instance AddrOffsetLe_refl z : AddrOffsetLe z z.
-Proof. apply Z.le_refl. Qed.
-
-Lemma AddrOffsetLe_compute z z': (z <=? z' = true)%Z -> AddrOffsetLe z z'.
-Proof. intro. apply Z.leb_le; auto. Qed.
-#[export] Hint Extern 1 (AddrOffsetLe _ _) => (apply AddrOffsetLe_compute; reflexivity) : typeclass_instances.
-
-Lemma AddrOffsetLt_compute z z': (z <? z' = true)%Z -> AddrOffsetLt z z'.
-Proof. intro. apply Z.ltb_lt; auto. Qed.
-#[export] Hint Extern 1 (AddrOffsetLt _ _) => (apply AddrOffsetLt_compute; reflexivity) : typeclass_instances.
-
-Instance AddrOffsetLe_of_lt z z': AddrOffsetLt z z' → AddrOffsetLe z z'.
-Proof. unfold AddrOffsetLt, AddrOffsetLe. lia. Qed.
-
-Instance AsWeakAddrIncr_incr b z:
-  AsWeakAddrIncr (b ^+ z)%a b z.
-Proof. reflexivity. Qed.
-
-Instance AsWeakAddrIncr_no_incr b :
-  AsWeakAddrIncr b b 0 | 50.
-Proof. unfold AsWeakAddrIncr. solve_addr. Qed.
-
-Instance AddrLe_refl a : AddrLe a a.
-Proof. unfold AddrLe. solve_addr. Qed.
-
-Instance AddrLe_of_lt a a' : AddrLt a a' → AddrLe a a'.
-Proof. unfold AddrLt, AddrLe. solve_addr. Qed.
-
-Instance AddrLe_offsets (a a' a'': Addr) (z z': Z) :
-  AsWeakAddrIncr a' a z →
-  AsWeakAddrIncr a'' a z' →
-  AddrOffsetLe 0 z →
-  AddrOffsetLe z z' →
-  AddrLe a' a''.
-Proof. unfold AddrOffsetLe, AddrLe, AsWeakAddrIncr. solve_addr. Qed.
-
-Instance AddrLt_offsets (a a' a'': Addr) (z z': Z) :
-  AsWeakAddrIncr a' a z →
-  AsWeakAddrIncr a'' a z' →
-  AddrOffsetLe 0 z →
-  ContiguousRegion a z' →
-  AddrOffsetLt z z' →
-  AddrLt a' a''.
-Proof.
-  unfold AsWeakAddrIncr, AddrOffsetLe, AddrOffsetLt, AddrLt.
-  intros ? ? ? [? ?] ?. solve_addr.
-Qed.
-
-Instance AddrEqSame a : AddrEq a a true.
-Proof. constructor. Qed.
-
-Instance AddrEq_offset_cbv b z z' :
-  CbvTC z z' →
-  AddrEq (b ^+ z)%a (b ^+ z')%a true.
-Proof. intros ->. constructor. Qed.
-
-Instance AddrEq_default_neq a a' : AddrEq a a' false | 100.
-Proof. inversion 1. Qed.
-
-Instance ZToAddr_z_of a :
-  ZToAddr (z_of a) a.
-Proof. apply finz_of_z_to_z. Qed.
-
-(* other *)
+From machine_utils Require Export class_instances.
 
 Instance DecodeInstr_encode `{MachineParameters} (i: instr) :
   DecodeInstr (encodeInstrW i) i.
 Proof. apply decode_encode_instrW_inv. Qed.
-
-
-
-
-(* Tests *)
-
-Goal forall (a: Addr),
-  AddrEq (a ^+ 1)%a (a ^+ (Z.of_nat 1))%a true.
-Proof. typeclasses eauto. Qed.
-
-Goal forall (a: Addr), exists a' z,
-  AsWeakAddrIncr (a ^+ 1)%a a' z ∧ a' = a ∧ z = 1%Z.
-Proof. intros. do 2 eexists. repeat apply conj. typeclasses eauto. all: reflexivity. Qed.
 
